add repeat[i]_blocks and loop[i]_blocks

code/experimental/sha3/Hacl.Impl.SHA3.fst
@@ -196,13 +196,13 @@ let state_pi_rho s =
   let current:lbuffer uint64 1 = create (size 1) (readLane s (size 1) (size 0)) in
   let h1 = ST.get () in
   assert (bget h1 current 0 == S.readLane (as_seq h0 s) 1 0);
-  [@ inline_let]  
+  [@ inline_let]
   let a_impl = (lbuffer uint64 1) & state in
-  [@ inline_let]  
+  [@ inline_let]
   let refl h i : GTot (uint64 & S.state) = get h current 0, as_seq h s in
-  [@ inline_let]  
+  [@ inline_let]
   let footprint i = loc_union (loc_buffer current) (loc_buffer s) in
-  [@ inline_let]  
+  [@ inline_let]
   let spec h0 = S.state_pi_rho_inner in
   let h0 = ST.get () in
   loop h0 (size 24) S.state_pi_rho_s a_impl (current, s) refl footprint spec
@@ -458,14 +458,11 @@ val absorb:
       S.absorb (as_seq h0 s) (v rateInBytes) (v inputByteLen)
         (as_seq h0 input) delimitedSuffix)
 let absorb s rateInBytes inputByteLen input delimitedSuffix =
-  [@ inline_let]
-  let spec_f = (fun i -> S.absorb_inner (v rateInBytes)) in
-  [@ inline_let]
-  let spec_l = (fun i -> S.absorb_last delimitedSuffix (v rateInBytes)) in
   loop_blocks rateInBytes inputByteLen input
-  spec_f spec_l
-  (fun i -> absorb_inner rateInBytes)
-  (fun i -> absorb_last delimitedSuffix rateInBytes) s
+  (S.absorb_inner (v rateInBytes))
+  (S.absorb_last delimitedSuffix (v rateInBytes))
+  (absorb_inner rateInBytes)
+  (absorb_last delimitedSuffix rateInBytes) s
 
 #reset-options "--z3rlimit 50 --max_fuel 0 --max_ifuel 1"
 
@@ -537,21 +534,21 @@ let squeeze s rateInBytes outputByteLen output = admit(); //TODO: add loop2
   let outBlocks = outputByteLen /. rateInBytes in
   let remOut = outputByteLen %. rateInBytes in
   let tmp = sub output (outputByteLen -. remOut) remOut in
-  [@ inline_let]  
+  [@ inline_let]
   let a_spec (i:size_nat{i <= v outputByteLen / v rateInBytes}) =
     S.state & (LB.lbytes (i * v rateInBytes)) in
-  [@ inline_let]    
+  [@ inline_let]
   let a_impl = state & (lbytes (v outputByteLen)) in
-  [@ inline_let]  
+  [@ inline_let]
   let refl h (i:size_nat{i <= v outBlocks}) :
     GTot (S.state & (LB.lbytes (i * v rateInBytes))) =
     assert (i * v rateInBytes <= v outputByteLen);
     as_seq h s,
     as_seq h (gsub output (size 0) (size i *! rateInBytes))
   in
-  [@ inline_let]  
+  [@ inline_let]
   let footprint i = loc_union (loc_buffer s) (loc_buffer output) in
-  [@ inline_let]  
+  [@ inline_let]
   let spec h0: i:size_nat{i < v outBlocks} -> a_spec i -> a_spec (i + 1) =
     S.squeeze_inner (v rateInBytes) (v outputByteLen) in
   let h0 = ST.get () in
